\centers{\question{Alternative representation}}

\noindent
Another expression for the variance might be

\centers{$ \f{ \ddot{\lambda}(-1) - { \dot{\lambda}(-1) }^2 }{ { \dot{\lambda}(-1) }^3 } $}

\noindent I was able to compute this coefficient for a Markov chain of size 2. It 
might be applied to the general case~$n$ by solving a linear system of the same size
and computing an approximation of the largest eigenvalue $\lambda$. 

\leftcenters
    {In the paper,}
    {$ \ddot{\lambda}(-1) = \pi \ddot{P}(-1)\psi
                        + 2 \dot{\pi}(-1) \dot{P}(-1) \psi
                        - 2 \dot{\lambda}(-1) \dot{\pi}(-1) \psi $}


\noindent First term is
\centers
    { $\pi_0 \, p_{0 0} \, \log^2 (p_{0 0}) 
        + \pi_1 \, p_{1 0} \, \log^2 (p_{1 0}) 
        + \pi_0 \, p_{0 1} \, \log^2 (p_{0 1}) 
        + \pi_1 \, p_{1 1} \, \log^2 (p_{1 1})  $}

\noindent The second is
\centers
    { $ - 2 \pac{
            \dot{\pi}_0(-1) p_{0 0} \log (p_{0 0})    
            + \dot{\pi}_1(-1) p_{1 0} \log (p_{1 0}) 
            + \dot{\pi}_0(-1) p_{0 1} \log (p_{0 1})
            + \dot{\pi}_1(-1) p_{1 1} \log (p_{1 1})
        }   
    $}

\noindent The third is
\centers{
    $ - 2 \dot{\lambda}(-1) \pac{
        \dot{\pi}_0(-1) 
        + \dot{\pi}_1(-1)
    }$
}

\noindent We 
        have to compute $\dot{\pi}(-1)$. With 
            $\pi(s) = (\pi_0(s), \, \pi_1(s))$, and since

\centers{$\pi(s) P(s) = \lambda(s) \pi(s)$}

\leftcenters
    {then we have}
    {$ \left\{
        \begin{aligned}
            {p_{0 0}}^{-s} \pi_0(s) + {p_{0 1}}^{-s} \pi_1(s) &= \lambda(s) \pi_0(s) \\
            {p_{1 0}}^{-s} \pi_0(s) + {p_{1 1}}^{-s} \pi_1(s) &= \lambda(s) \pi_1(s) \\
        \end{aligned}
        \right.
     $}

which I'm not sure how to solve formally.
% \noindent
% solving for $\pi_0(s)$ and $\pi_1(s)$, 
% assuming $ p_{0 0} p_{1 1} \neq p_{0 1} p_{1 0} $ :

% \centers{$ \pi_0(s) = \lambda(s) \f{ \overbrace{{p_{1 1}}^{-s} - {p_{0 1}}^{-s}}^{g_0(s)} }
%                                    { \underbrace{{ (p_{0 0} p_{1 1}) }^{-s} 
%                                         - { (p_{0 1} p_{1 0}) }^{-s}}_{\delta(s)} }
%             \qquad 
%             \text{and}
%             \qquad
%        \pi_1(s) = \lambda(s) \f{ \overbrace{{p_{0 0}}^{-s} - {p_{1 0}}^{-s}}^{g_1(s)} }
%                                    { { (p_{0 0} p_{1 1}) }^{-s} 
%                                         - { (p_{0 1} p_{1 0}) }^{-s} }$}


% \leftcenters
%     {hence for $i\in\{0,1\}$}
%     {$ \dot{\pi}_i(s) = \dot{\lambda}(s) \f{g_i(s)}{\delta(s)}
%                         + \lambda(s) \f{{g_i}'(s)\delta(s) - g_i(s)\delta'(s)}
%                                         {\delta^2(s)}$}

% \leftcenters
%     {so}
%     {$ \dot{\pi}_i(-1) = h \f{g_i(-1)}{\delta(-1)}
%                         + \f{{g_i}'(-1) \delta(-1) - g_i(-1) \delta'(-1) }
%                             {\delta^2(-1)} $}

% \begin{egalites}
%     with & \delta(-1) 
%             & p_{0 0} p_{1 1} - p_{0 1} p_{1 0} \\[3mm]
%          &g_0(-1) 
%             & p_{1 1} - p_{0 1} \\[3mm]
%         &{g_0}'(-1)
%             & -\ln (p_{1 1}) p_{1 1} + \ln (p_{0 1}) p_{0 1} \\[3mm]
%         &g_1(-1)
%             & p_{0 0} - p_{1 0} \\[3mm]
%         &{g_1}'(-1) 
%             & -\ln (p_{0 0}) p_{0 0} + \ln (p_{1 0}) p_{1 0} 
% \end{egalites}


% \leftcenters
%     {where}
%     {  $\left\{
%         \begin{minipage}{0.6\textwidth}
%        $ {g_0}'(s) = - \ln(p_{1 1}) {p_{1 1}}^{-s}
%                  + \ln(p_{0 1}) {p_{0 1}}^{-s}$ \\[3mm]
%         $\delta'(s) = - \ln( p_{0 0} p_{1 1}) { (p_{0 0} p_{1 1}) }^{-s}
%                         +  \ln ( p_{0 1} p_{1 0} ) { (p_{0 1} p_{1 0}) }^{-s} $
%         \end{minipage}
%         \right.$ }



% \noindent
% Now taking $s=-1$ and re-arranging in a linear system of unknown $\dot{\pi}_0(-1)$ and $\dot{\pi}_1(-1)$ :
% \centers
%     {$ \left\{
%         \begin{aligned}
%             \dot{\pi}_0(-1) (p_{0 0} - \lambda)
%             + \dot{\pi}_1(-1) p_{0 1}
%                 &= \dot{\lambda}(-1) \pi_0
%                     +   \ln p_{0 0} \cdot p_{0 0} \pi_0
%                     +   \ln p_{0 1} \cdot p_{0 1} \pi_1 \\
%             \dot{\pi}_0(-1) p_{1 0}
%             + \dot{\pi}_1(-1) (p_{1 1} - \lambda)
%                 &= \dot{\lambda}(-1) \pi_1
%                     +  \ln p_{1 0} \cdot p_{1 0} \pi_0 
%                     +  \ln p_{1 1} \cdot p_{1 1} \pi_1
%         \end{aligned}
%         \right.
%      $}

% \noindent since
% $\dot{\lambda}(-1) = h$ and,
% $\lambda(-1) = 1$ :

% \centers
%     {$ \left\{
%         \begin{aligned}
%             \dot{\pi}_0(-1) (p_{0 0} - 1)
%             + \dot{\pi}_1(-1) p_{0 1}
%                 &= h \pi_0
%                     +   \ln p_{0 0} \cdot p_{0 0} \pi_0
%                     +   \ln p_{0 1} \cdot p_{0 1} \pi_1 \\
%             \dot{\pi}_0(-1) p_{1 0}
%             + \dot{\pi}_1(-1) (p_{1 1} - 1)
%                 &= h \pi_1
%                     +  \ln p_{1 0} \cdot p_{1 0} \pi_0 
%                     +  \ln p_{1 1} \cdot p_{1 1} \pi_1
%         \end{aligned}
%         \right.
%      $}

% \begin{egalites}
% which is  &\lambda
%         &\f{ (p_{0 0} + p_{1 1}) 
%            + \sqrt{ (p_{0 0} + p_{1 1})^2 - 4 (p_{0 0} p_{1 1} - p_{1 0} p_{0 1}) }}
%            {2}\\[3mm]
%         &&\f{ (p_{0 0} + p_{1 1}) 
%            + \sqrt{ (p_{0 0} - p_{1 1})^2 + 4 p_{1 0} p_{0 1} }}
%            {2}   
% \end{egalites}




