\newtheorem{Definition}{def}

\question{Notations}

\begin{def}
Let $W$ be the random variable which outputs words of length $n$ 
(of $\Omega_n$) from a memoryless source.
\end{def}

\begin{def}
 Let $J \in \mathbb{N}^{\star}$ be a random
variable which, for every word $w$, uniformly picks the index of
one of its phrases. The joint law of $J$ with $W$ is :

\centers{$ \proba{ W=w, J=j } = 
                    \left\{ \begin{array}{l}
                        \tf{1}{M_n(w)} \quad \textmd{ if } j \leq M_n(w) \\
                        0 \qquad \qquad \textmd{ else }
                    \end{array}
                    \right. $ }
\end{def}

\begin{def}
The function defined as $g$ is a random variable that depends on $W$, therefore
we write it as $g_W$, or, during the event $\{ W=w \}$, $g_w$. 
Samely, we will study the random variable $g_W(J)$, and will
sometimes write $g_w(j)$ when both the events $[W=w]$ and $[J=j]$
occur.


\leftcenters
    {We define the random variable}
    {$B_{J, W}^k = | L_{g_W(J) - k} |$}

\noindent
and we will study the random variable
    {$ \underset{ 0 \leq k \leq g_W(J) }{ \max } 
                    \left\{ { B_{J, W}^k - k } \right\} $}

\noindent
For $J = j$, $W = w$ and $j \leq M_n(w)$, this random variable is the length of 
the $j^{\textmd{th}}$ phrase of the flexible parsing of the word $w$. We have,
accordingly,

\centers{$ D_n^{FLEX} (w) = \f{1}{M_n(w)} \Sum{j=0}{M_n(w)-1} |u_j^{FLEX}|
                          = \f{1}{M_n(w)} \Sum{j=0}{M_n(w)-1}  
                                \underset{ 0 \leq k \leq g_w(j) }{ \max } 
                                \left\{ { B_{j, w}^k - k } \right\} $}
\noindent
Precisely, $D_n^{FLEX}(w)$ is the empirical average of the lengths of the phrases
of the flexible parsing of a word $w$, whereas 
        $\underset{ 0 \leq k \leq g_w(J) }{ \max } 
        \left\{ { B_{J, w}^k - k } \right\} $,
with $J$ a random variable and $w$ fixed,
is the length of a uniformly randomly selected phrase of the flexible parsing
of $w$. 

\leftcenters   
    {Finally, we define}
    {$x_n = \f1{h} \log_2 \pa{ \f{nh}{\log_2(n)} }$}

\leftcenters
    {as well as}
    {$b_n^{\delta} = x_n + (c_3 x_n)^{\delta}$}

\leftcenters
    {and we study}
    {$ \proba{ 
        \underset{ 0 \leq k \leq g_w(J) }{ \max } 
        \left\{ { B_{J, w}^k - k } \right\}
            > b_n^{\delta} } $}